Kami/Ex/Timing/LabelDecomposition.v
@@ -1,0 +1,58 @@
+Require Import Bool List String Omega.
+Require Import Structures.Equalities Program.Equality Eqdep Eqdep_dec.
+Require Import FunctionalExtensionality.
+Require Import Lib.Word Lib.CommonTactics Lib.ilist Lib.FMap Lib.StringEq Lib.VectorFacts Lib.Struct.
+Require Import Kami.Syntax Kami.Semantics Kami.Decomposition.
+
+Section GivenModule.
+  Variable m: Modules.
+
+  Section GivenOldregs.
+    Variable o: RegsT.
+
+    Variable Prule : MethsT -> Prop.
+    Variable Pmeth : MethsT -> Prop.
+
+    Example rqMeth := "rqFromProc" : String.string.
+    Example rsMeth := "rsToProc" : String.string.
+    Example Qrule := fun cs => FMap.M.find (elt := {x : SignatureT & SignT x}) rqMeth cs = None \/
+                            FMap.M.find (elt := {x : SignatureT & SignT x}) rsMeth cs = None.
+    Example Qmeth := fun cs => FMap.M.find (elt := {x : SignatureT & SignT x}) rqMeth cs = None /\
+                            FMap.M.find (elt := {x : SignatureT & SignT x}) rsMeth cs = None.
+
+    Axiom Prule_empty : Prule ([])%fmap.
+   
+    Axiom Prules : forall k a, List.In {| attrName := k; attrType := a |} (getRules m) ->
+                          forall u cs retVal, SemAction o (a type) u cs retVal ->
+                                         Prule cs.
+    Axiom Pmeths :  forall f, In f (getDefsBodies m) ->
+                         forall (u : UpdatesT) (cs : MethsT) (argV : type (arg (projT1 (attrType f)))) (retV : type (ret (projT1 (attrType f)))),
+                           SemAction o (projT2 (attrType f) type argV) u cs retV ->
+                           Pmeth cs.
+
+    Axiom Pmeru : forall rcs, Prule rcs ->
+                         forall mcs, Pmeth mcs ->
+                                Prule (M.union rcs mcs).
+    
+    
+    Goal forall u l, Step m o u l -> Prule (calls l).
+      induction 1. unfold hide.
+      induction ss; simpl.
+      - match goal with
+          [ |- Prule ?x ] => idtac x; change x with (@M.Map.empty {z : SignatureT & SignT z})
+        end; apply Prule_empty.
+      - destruct a. assert (Prule cms).
+        { destruct substep.
+          + apply Prule_empty.
+          + apply Prule_empty.
+          + eapply Prules; eassumption.
+          + replace (cs) with (M.union [] cs)%fmap by (apply M.union_empty_L).
+            eapply Pmeru. apply Prule_empty.
+            eapply Pmeths; eassumption.
+        }
+        simpl in IHss. inv HSubsteps. specialize (IHss H2). simpl in HWellHidden.
+
+        (*unfold wellHidden in HWellHidden.
+        RefinementFacts.DomainSubset_KeysDisj*)
+        
+                                        
