Kami/Ex/Timing/ThreeStageInterface.v
@@ -7,8 +7,12 @@ Require Import Ex.Timing.Specification.
 Require Import Lib.CommonTactics.
 
 
+Definition rv32iRq := RqFromProc rv32iAddrSize rv32iDataBytes.
+Definition rv32iRs := RsToProc rv32iDataBytes.
+  
 
 Module Type ThreeStageInterface.
+
   Parameter p : Modules.
   Parameter m : Modules.
 
@@ -23,7 +27,7 @@ Module Type ThreeStageInterface.
   Axiom callsDisj : FMap.DisjList (getCalls p) (getCalls m).
 
   Parameter ThreeStageProcRegs : regfile -> progMem -> address -> RegsT.
-  Parameter ThreeStageMemRegs : memory -> RegsT.
+  Parameter ThreeStageMemRegs : memory -> data -> RegsT.
 
   Parameter fhMeth : String.string.
   Parameter thMeth : String.string.
@@ -43,16 +47,419 @@ Module Type ThreeStageInterface.
   Axiom mndth : ~ In thMeth (getDefs m).
 
   Axiom pRegs : forall rf pm pc, FMap.M.KeysSubset (ThreeStageProcRegs rf pm pc) (Struct.namesOf (getRegInits p)).
-  Axiom mRegs : forall mem, FMap.M.KeysSubset (ThreeStageMemRegs mem) (Struct.namesOf (getRegInits m)).
+  Axiom mRegs : forall mem nextRs, FMap.M.KeysSubset (ThreeStageMemRegs mem nextRs) (Struct.namesOf (getRegInits m)).
 
   Axiom pRqRs : forall rf u l,
       Step p rf u l ->
       (FMap.M.find rqMeth (calls l) = None \/
        FMap.M.find rsMeth (calls l) = None).
 
-  Axiom mRqRs : forall rf u l,
-      Step m rf u l ->
-      (FMap.M.find rqMeth (defs l) = None \/
-       FMap.M.find rsMeth (defs l) = None).
+  Axiom mRqRs : forall rp rm up um lp lm,
+      Step p rp up lp ->
+      Step m rm um lm ->
+      WellHiddenConcat p m lp lm -> 
+      (FMap.M.find rqMeth (defs lm) = None \/
+       FMap.M.find rsMeth (defs lm) = None).
 
+
+  
 End ThreeStageInterface.
+
+Module ThreeStageDefs (ThreeStage : ThreeStageInterface).
+  Import ThreeStage.
+  
+  Definition censorThreeStageLabel (lastRq : option bool) censorMeth (l : LabelT) := censorLabel (censorMeth lastRq) l.
+   
+  Definition censorThreeStageMeth (lastRqOp : option bool) (n : String.string) (t : {x : SignatureT & SignT x}) : {x : SignatureT & SignT x} :=
+    if String.string_dec n rqMeth
+    then match t with
+         | existT _
+                  {| arg := Struct (STRUCT {"addr" :: Bit 16;
+                                            "op" :: Bool;
+                                            "data" :: Bit 32});
+                     ret := Bit 0 |}
+                  (argV, retV) =>
+           let op := evalExpr (#argV!rv32iRq@."op")%kami_expr in
+           existT _
+                  {| arg := Struct (STRUCT {"addr" :: Bit 16;
+                                            "op" :: Bool;
+                                            "data" :: Bit 32});
+                     ret := Bit 0 |}
+                  (evalExpr (STRUCT {"addr" ::= #argV!rv32iRq@."addr";
+                                       "op" ::=  #argV!rv32iRq@."op";
+                                     "data" ::= if op
+                                                then $0
+                                                else #argV!rv32iRq@."data"})%kami_expr,
+                   evalExpr ($$WO)%kami_expr)
+         | _ => t
+         end
+    else if String.string_dec n rsMeth
+         then match t with
+         | existT _
+                  {| arg := Bit 0;
+                     ret := Struct (STRUCT {"data" :: Bit 32}) |}
+                  (argV, retV) =>
+           existT _
+                  {| arg := Bit 0;
+                     ret := Struct (STRUCT {"data" :: Bit 32}) |}
+                  (evalExpr ($$WO)%kami_expr,
+                   evalExpr (STRUCT {"data" ::= match lastRqOp with
+                                                | Some op => if op
+                                                           then #retV!rv32iRs@."data"
+                                                           else $0
+                                                | None => #retV!rv32iRs@."data"
+                                                end})%kami_expr)
+         | _ => t
+              end 
+         else if String.string_dec n thMeth
+              then match t with
+                   | existT _
+                            {| arg := Bit 32;
+                               ret := Bit 0 |}
+                            (argV, retV) =>
+                     existT _
+                       {| arg := Bit 32;
+                          ret := Bit 0 |}
+                       ($0, retV)
+                   | _ => t
+                   end
+              else if String.string_dec n fhMeth
+                   then match t with
+                        | existT _
+                                 {| arg := Bit 0;
+                                    ret := Bit 32 |}
+                                 (argV, retV) =>
+                          existT _
+                                 {| arg := Bit 0;
+                                    ret := Bit 32 |}
+                                 (argV, $0)
+                        | _ => t
+                        end
+                   else t.
+
+    Definition censorThreeStageMemDefs (lastRqOp : option bool) (n : String.string) (t : {x : SignatureT & SignT x}) : {x : SignatureT & SignT x} :=
+    if String.string_dec n rqMeth
+    then match t with
+         | existT _
+                  {| arg := Struct (STRUCT {"addr" :: Bit 16;
+                                            "op" :: Bool;
+                                            "data" :: Bit 32});
+                     ret := Bit 0 |}
+                  (argV, retV) =>
+           let op := evalExpr (#argV!rv32iRq@."op")%kami_expr in
+           existT _
+                  {| arg := Struct (STRUCT {"addr" :: Bit 16;
+                                            "op" :: Bool;
+                                            "data" :: Bit 32});
+                     ret := Bit 0 |}
+                  (evalExpr (STRUCT {"addr" ::= #argV!rv32iRq@."addr";
+                                     "op" ::=  #argV!rv32iRq@."op";
+                                     "data" ::= if op
+                                                then $0
+                                                else #argV!rv32iRq@."data"})%kami_expr,
+                   evalExpr ($$WO)%kami_expr)
+         | _ => t
+         end
+    else if String.string_dec n rsMeth
+         then match t with
+         | existT _
+                  {| arg := Bit 0;
+                     ret := Struct (STRUCT {"data" :: Bit 32}) |}
+                  (argV, retV) =>
+           existT _
+                  {| arg := Bit 0;
+                     ret := Struct (STRUCT {"data" :: Bit 32}) |}
+                  (evalExpr ($$WO)%kami_expr,
+                   evalExpr (STRUCT {"data" ::= match lastRqOp with
+                                                | Some op => if op
+                                                            then #retV!rv32iRs@."data"
+                                                            else $0
+                                                | None => #retV!rv32iRs@."data"
+                                                end})%kami_expr)
+         | _ => t
+              end
+         else t.
+
+  
+  Definition getRqCall (lastRq : option bool) (l : LabelT) : option bool:=
+    match FMap.M.find rqMeth (calls l) with
+    | Some (existT _
+                     {| arg := Struct (STRUCT {"addr" :: Bit 16;
+                                               "op" :: Bool;
+                                               "data" :: Bit 32});
+                        ret := Bit 0 |}
+                     (argV, retV)) =>
+      Some (evalExpr (#argV!rv32iRq@."op")%kami_expr)
+    | _ => match FMap.M.find rsMeth (calls l) with
+          | Some _ => None
+          | None => lastRq  (* nothing memory-relevant happened this cycle *)
+          end
+    end.
+
+  Definition getRqDef (lastRq : option bool) (l : LabelT) : option bool :=
+    match FMap.M.find rqMeth (defs l) with
+    | Some (existT _
+                     {| arg := Struct (STRUCT {"addr" :: Bit 16;
+                                               "op" :: Bool;
+                                               "data" :: Bit 32});
+                        ret := Bit 0 |}
+                     (argV, retV)) =>
+      Some (evalExpr (#argV!rv32iRq@."op")%kami_expr)
+    | _ => match FMap.M.find rsMeth (defs l) with
+          | Some _ => None
+          | None => lastRq
+          end
+    end.
+
+
+  Fixpoint censorThreeStageLabelSeq (lastRq: option bool) getRqMeth censorMeth (ls : LabelSeqT) {struct ls} : LabelSeqT :=
+    match ls with
+    | nil => nil
+    | l :: ls' => 
+      (censorLabel (censorMeth lastRq) l) :: censorThreeStageLabelSeq (getRqMeth lastRq l) getRqMeth censorMeth ls'
+    end.
+      
+  Inductive ThreeStageProcMemConsistent : LabelSeqT -> option (bool * address) -> memory -> Prop := (* unclear what this becomes if calls aren't well-balanced, or whether that matters *)
+  | S3PMCnil : forall lastRq mem, ThreeStageProcMemConsistent nil lastRq mem
+  | S3PMCrq : forall (lastRq :option(bool*address)) mem l last' mem' ls argV retV,
+      (FMap.M.find rqMeth (calls l) = Some (existT _
+                                                   {| arg := Struct (STRUCT {"addr" :: Bit 16;
+                                                                             "op" :: Bool;
+                                                                             "data" :: Bit 32});
+                                                      ret := Bit 0 |}
+                                                   (argV, retV)) /\
+       let addr := evalExpr (#argV!rv32iRq@."addr")%kami_expr in
+       let argval := evalExpr (#argV!rv32iRq@."data")%kami_expr in
+       let op := evalExpr (#argV!rv32iRq@."op")%kami_expr in
+       last' = Some (op, addr) /\
+       if op
+       then mem' = (fun a => if weq a addr then argval else mem a) (* ST *)
+       else mem' = mem (* LD *)) ->
+      ThreeStageProcMemConsistent ls last' mem' ->
+      ThreeStageProcMemConsistent (l :: ls) lastRq mem
+  | S3PMCrs : forall (lastRq :option(bool*address)) mem l last' mem' ls argV retV,
+      (FMap.M.find rsMeth (calls l) = Some (existT _
+                                                   {| arg := Bit 0;
+                                                      ret := Struct (STRUCT {"data" :: Bit 32})|}
+                                                   (argV, retV)) /\
+       last' = None /\ 
+       match lastRq with
+       | Some (op, addr) =>
+         if op
+         then (* previous request was a ST *)
+           mem' = mem (* we already did the update immediately upon getting the request *)
+         else (* previous request was "LD addr" *)
+           let retval := evalExpr (#retV!rv32iRs@."data")%kami_expr in
+           mem' = mem /\ mem addr = retval
+       | _ => (* this is the non-well-balanced case, not sure what goes here *)
+         mem' = mem 
+       end) ->
+      ThreeStageProcMemConsistent ls last' mem' ->
+      ThreeStageProcMemConsistent (l :: ls) lastRq mem
+  | S3PMCcons : forall (lastRq :option(bool*address)) mem l last' mem' ls, 
+      (FMap.M.find rqMeth (calls l) = None
+       /\ FMap.M.find rsMeth (calls l) = None
+       /\ mem' = mem /\ last' = lastRq) -> 
+      ThreeStageProcMemConsistent ls last' mem' ->
+      ThreeStageProcMemConsistent (l :: ls) lastRq mem.
+  
+  Definition ThreeStageProcHiding m (lastRq : option (bool * address)) regs mem : Prop := 
+    forall labels newRegs fhs,
+      ForwardMultistep m regs newRegs labels ->
+      ThreeStageProcMemConsistent labels lastRq mem ->
+      extractFhLabelSeq fhMeth labels = fhs ->
+      forall fhs',
+        length fhs = length fhs' ->
+        exists labels' newRegs',
+          ForwardMultistep m regs newRegs' labels' /\
+          ThreeStageProcMemConsistent labels' lastRq mem /\
+          censorThreeStageLabelSeq (option_map fst lastRq) getRqCall censorThreeStageMeth labels = censorThreeStageLabelSeq (option_map fst lastRq) getRqCall censorThreeStageMeth labels' /\
+          extractFhLabelSeq fhMeth labels' = fhs'.
+
+  Definition ThreeStageProcLabelAirtight (l : LabelT) : Prop :=
+    match FMap.M.find rqMeth (calls l) with
+    | Some (existT _
+                   {| arg := Struct (STRUCT {"addr" :: Bit 16;
+                                             "op" :: Bool; 
+                                             "data" :: Bit 32});
+                      ret := Bit 0 |}
+                   (argV, _)) =>
+      if evalExpr (#argV!rv32iRq@."op")%kami_expr
+      then True (* ST *)
+      else evalExpr (#argV!rv32iRq@."data")%kami_expr = $0 (* LD *)
+    | _ => True
+    end. (* Guarantees the _processor_ doesn't leak over the unused fields. *)
+  
+  Definition ThreeStageProcLabelSeqAirtight : LabelSeqT -> Prop := Forall ThreeStageProcLabelAirtight.
+
+
+  Definition extractMethsWrVals (ms : MethsT) : list (word 32) :=
+    match FMap.M.find rqMeth ms with
+    | Some (existT _
+                   {| arg := Struct (STRUCT {"addr" :: Bit 16;
+                                             "op" :: Bool;
+                                             "data" :: Bit 32});
+                      ret := Bit 0 |}
+                   (argV, retV)) =>
+      if evalExpr (#argV!rv32iRq@."op")%kami_expr
+      then [evalExpr (#argV!rv32iRq@."data")%kami_expr]
+      else nil
+    | _ => nil
+    end.
+
+  Definition extractMethsRdVals (lastRq : option bool) (ms : MethsT) : list (word 32) :=
+    match FMap.M.find rsMeth ms with
+    | Some (existT _
+                   {| arg := Bit 0;
+                      ret := Struct (STRUCT {"data" :: Bit 32}) |}
+                   (argV, retV)) =>
+      match lastRq with
+      | Some op => 
+        if op
+        then nil
+        else [evalExpr (#retV!rv32iRs@."data")%kami_expr]
+      | _ => nil
+      end
+    | _ => nil
+    end.
+  
+  Definition extractProcWrValSeq : LabelSeqT -> list (word 32) :=
+    flat_map (fun l => extractMethsWrVals (calls l)).
+  
+  Definition extractMemWrValSeq : LabelSeqT -> list (word 32) :=
+    flat_map (fun l => extractMethsWrVals (defs l)).
+
+  Fixpoint extractProcRdValSeq (lastRq : option bool) (ls :  LabelSeqT) : list (word 32) :=
+    match ls with
+    | nil => nil
+    | l :: ls' => (extractMethsRdVals lastRq (calls l)) ++ extractProcRdValSeq (getRqCall lastRq l) ls' 
+    end.
+
+
+  Fixpoint extractMemRdValSeq (lastRq : option bool) (ls :  LabelSeqT) : list (word 32) :=
+    match ls with
+    | nil => nil
+    | l :: ls' => (extractMethsRdVals lastRq (defs l)) ++ extractMemRdValSeq (getRqDef lastRq l) ls' 
+    end.
+  
+  Inductive ThreeStageMemMemConsistent : LabelSeqT -> option (bool * address) -> memory -> Prop := 
+  | S3MMCnil : forall lastRq mem, ThreeStageMemMemConsistent nil lastRq mem
+  | S3MMCrq : forall (lastRq:option(bool*address)) mem l last' mem' ls argV retV,
+      (FMap.M.find rqMeth (defs l) = Some (existT _
+                     {| arg := Struct (STRUCT {"addr" :: Bit 16;
+                                               "op" :: Bool;
+                                               "data" :: Bit 32});
+                        ret := Bit 0 |}
+                     (argV, retV)) /\
+                    let addr := evalExpr (#argV!rv32iRq@."addr")%kami_expr in
+                    let argval := evalExpr (#argV!rv32iRq@."data")%kami_expr in
+                    let op := evalExpr (#argV!rv32iRq@."op")%kami_expr in
+                    last' = Some (op, addr) /\
+                    if op
+                    then mem' = (fun a => if weq a addr then argval else mem a) (* ST *)
+                    else mem' = mem (* LD *)
+      ) ->
+      ThreeStageMemMemConsistent ls last' mem' ->
+      ThreeStageMemMemConsistent (l :: ls) lastRq mem
+  | S3MMCrs : forall (lastRq:option(bool*address)) mem l last' mem' ls argV retV,
+      (FMap.M.find rsMeth (defs l) = Some (existT _
+                                                  {| arg := Bit 0;
+                                                     ret := Struct (STRUCT {"data" :: Bit 32})|}
+                                                  (argV, retV)) /\
+       last' = None /\ match lastRq with
+                      | Some (op, addr) =>
+                        if op
+                        then (* previous request was a ST *)
+                          mem' = mem (* we already did the update immediately upon getting the request *)
+                        else (* previous request was "LD addr" *)
+                          let retval := evalExpr (#retV!rv32iRs@."data")%kami_expr in
+                          mem' = mem /\ mem addr = retval
+                      | _ => (* this is the non-well-balanced case, not sure what goes here *)
+                        mem' = mem 
+                      end)      ->
+      ThreeStageMemMemConsistent ls last' mem' ->
+      ThreeStageMemMemConsistent (l :: ls) lastRq mem
+  | S3MMCcons : forall (lastRq :option(bool*address)) mem l last' mem' ls,
+      (FMap.M.find rqMeth (defs l) = None /\ FMap.M.find rsMeth (defs l) = None /\
+       mem' = mem /\ last' = lastRq)
+      ->
+      ThreeStageMemMemConsistent ls last' mem' ->
+      ThreeStageMemMemConsistent (l :: ls) lastRq mem.
+
+  Definition ThreeStageMemHiding m : Prop :=
+    forall mem lastRq nextRs labels newRegs,
+      ThreeStageMemMemConsistent labels lastRq mem ->
+      (* compatibility between lastRq and nextRs? *)
+      ForwardMultistep m (ThreeStageMemRegs mem nextRs) newRegs labels ->
+      forall wrs,
+        extractMemWrValSeq labels = wrs ->
+        forall mem' nextRs' wrs',
+          length wrs = length wrs' ->
+          (* compatibility between lastRq and nextRs'? *)
+          exists labels' newRegs',
+            ForwardMultistep m (ThreeStageMemRegs mem' nextRs') newRegs' labels' /\
+            ThreeStageMemMemConsistent labels' lastRq mem' /\
+            censorThreeStageLabelSeq (option_map fst lastRq) getRqDef censorThreeStageMemDefs labels = censorThreeStageLabelSeq  (option_map fst lastRq) getRqDef censorThreeStageMemDefs labels' /\
+            extractMemWrValSeq labels' = wrs'.
+
+  Definition ThreeStageMemSpec m : Prop :=
+    forall oldRegs newRegs labels,
+      ForwardMultistep m oldRegs newRegs labels ->
+      forall mem nextRs,
+        oldRegs = ThreeStageMemRegs mem nextRs ->
+        exists lastRq,  (* compatibility? *)
+        ThreeStageMemMemConsistent labels lastRq mem.
+
+  Inductive ThreeStageMemLabelSeqAirtight : LabelSeqT -> option bool -> Prop :=
+  | S3MLSAnil : forall lastRq, ThreeStageMemLabelSeqAirtight nil lastRq
+  | S3MLSAcons : forall l ls (lastRq :option bool) last', (
+      (exists argV retV, FMap.M.find rqMeth (defs l) = Some (existT _
+                                                  {| arg := Struct (STRUCT {"addr" :: Bit 16;
+                                                                            "op" :: Bool;
+                                                                            "data" :: Bit 32});
+                                                     ret := Bit 0 |}
+                                                  (argV, retV))
+                    /\ let op := evalExpr (#argV!rv32iRq@."op")%kami_expr in
+                      last' = Some op
+      ) \/ (
+        exists argV retV, FMap.M.find rsMeth (defs l) = Some (existT _
+                                                                {| arg := Bit 0;
+                                                                   ret := Struct (STRUCT {"data" :: Bit 32})|}
+                                                                (argV, retV))
+                     /\ last' = None /\
+                     match lastRq with
+                     | Some op =>
+                       if op then evalExpr (#retV!rv32iRs@."data")%kami_expr = $0 else True
+                     | _ => evalExpr (#retV!rv32iRs@."data")%kami_expr = $0  (* being cautious *)
+                     end
+      ) \/ (
+        FMap.M.find rqMeth (defs l) = None /\ FMap.M.find rsMeth (defs l) = None /\ last' = lastRq
+      )) -> 
+      ThreeStageMemLabelSeqAirtight ls last' ->
+      ThreeStageMemLabelSeqAirtight (l :: ls) lastRq.
+  
+End ThreeStageDefs.
+
+Module Type ThreeStageModularHiding (ThreeStage : ThreeStageInterface).
+  Module Defs := ThreeStageDefs ThreeStage.
+  Import ThreeStage Defs.
+
+  Axiom abstractToProcHiding :
+    forall lastRq rf pm pc mem,
+      abstractHiding rf pm pc mem ->
+      ThreeStageProcHiding p lastRq (ThreeStageProcRegs rf pm pc) mem.
+
+  
+  Axiom ProcAirtight : forall oldregs newregs labels,
+      ForwardMultistep p oldregs newregs labels ->
+      ThreeStageProcLabelSeqAirtight labels.
+  
+  Axiom MemHiding : ThreeStageMemHiding m.
+
+  Axiom MemSpec : ThreeStageMemSpec m.
+
+  Axiom MemAirtight : forall oldregs newregs labels,
+      ForwardMultistep m oldregs newregs labels ->
+      ThreeStageMemLabelSeqAirtight labels None.
+
+End ThreeStageModularHiding.
